Major progress with helpers to seq optim

src/FrameStack/Optimisations/SeqDeadCode.v
@@ -1,7 +1,8 @@
-From CoreErlang.FrameStack Require Import SubstSemanticsLemmas
+From CoreErlang.FrameStack Require Export SubstSemanticsLemmas
                                           CIU
                                           CTX
                                           Compatibility.
+Require Export Basics.
 
 Import ListNotations.
 
@@ -36,9 +37,9 @@ end.
 
 Fixpoint is_safe_simple (e : Exp) : bool :=
 match e with
-| VVal (VLit _) => true
 | VVal (VFunId _) => false
-| VVal (VVar _) => true
+| VVal (VVar _)   => true
+| VVal _          => true
 | EExp (ECons e1 e2) => is_safe_simple e1 && is_safe_simple e2
 | EExp (ETuple l) => forallb is_safe_simple l
 | EExp (ECall (VVal (VLit (Atom modu))) (VVal (VLit (Atom func))) args) =>
@@ -82,10 +83,11 @@ Fixpoint seq_elim (e : Exp) : Exp :=
           let e2' := seq_elim e2 in
             if will_fail e1' then e1'
             else
-              match is_safe_simple e1', is_safe_simple e2' with
-              | true, _      => e2'
-              | false, true  => e1'
-              | false, false => ESeq e1' e2'
+              match is_safe_simple e1' (* , is_safe_simple e2' *) with
+              | true (* , _ *)      => e2'
+              (* | false, true  => e1' <- this only needs to be done
+                                          when using 'effect' *)
+              | false (* , false *) => ESeq e1' e2'
               end
       | ELetRec l ebody =>
           let l' := map (fun '(n, e0) => (n, seq_elim e0)) l in
@@ -97,17 +99,17 @@ Fixpoint seq_elim (e : Exp) : Exp :=
 (*   end *).
 
 Fixpoint size_val (v : Val) : nat :=
-  match v with
+  1 (* match v with
   | VNil => 1
   | VLit _ => 1
   | VPid _ => 1
   | VCons hd tl => 1 + size_val hd + size_val tl
-  | VTuple l => 1 + fold_left (fun acc v => acc + size_val v) l 0
-  | VMap pairs => 1 + fold_left (fun acc '(a,b) => acc + size_val a + size_val b) pairs 0
+  | VTuple l => 1 + list_sum (map size_val l)
+  | VMap pairs => 1 + list_sum (map (fun '(a, b) => size_val a + size_val b) pairs)
   | VVar _ => 1
   | VFunId _ => 1
   | VClos ext _ _ e => 1 + fold_left (fun acc '(_,_,e0) => acc + size_exp e0) ext 0 + size_exp e
-  end
+  end *)
 with size_exp (e : Exp) : nat :=
   match e with
   | VVal v => 1 + size_val v
@@ -116,41 +118,240 @@ with size_exp (e : Exp) : nat :=
 with size_nonval (nv : NonVal) : nat :=
   match nv with
     | EFun _ e => size_exp e
-    | EValues l => fold_left (fun acc e => acc + size_exp e) l 0
+    | EValues l => list_sum (map size_exp l)
     | ECons hd tl => size_exp hd + size_exp tl
-    | ETuple l => fold_left (fun acc e => acc + size_exp e) l 0
-    | EMap l => fold_left (fun acc '(a,b) => acc + size_exp a + size_exp b) l 0
-    | ECall m f l => size_exp m + size_exp f + fold_left (fun acc e => acc + size_exp e) l 0
-    | EPrimOp _ l => fold_left (fun acc e => acc + size_exp e) l 0
-    | EApp e l => size_exp e + fold_left (fun acc e => acc + size_exp e) l 0
-    | ECase e branches => size_exp e + fold_left (fun acc '(_,g,b) => acc + size_exp g + size_exp b) branches 0
+    | ETuple l => list_sum (map size_exp l)
+    | EMap l => list_sum (map (fun '(a, b) => size_exp a + size_exp b) l)
+    | ECall m f l => size_exp m + size_exp f + list_sum (map size_exp l)
+    | EPrimOp _ l => list_sum (map size_exp l)
+    | EApp e l => size_exp e + list_sum (map size_exp l)
+    | ECase e branches => size_exp e + list_sum (map (
+         fun '(p, g, e) => size_exp g + size_exp e
+       ) branches)
     | ELet _ e1 e2 => size_exp e1 + size_exp e2
     | ESeq e1 e2 => size_exp e1 + size_exp e2
-    | ELetRec l e => fold_left (fun acc '(_,e0) => acc + size_exp e0) l 0 + size_exp e
+    | ELetRec l e => list_sum (map (fun '(_, a) => size_exp a) l) + size_exp e
     | ETry e1 _ e2 _ e3 => size_exp e1 + size_exp e2 + size_exp e3
   end.
+
+Ltac do_step := econstructor; [constructor;auto| simpl].
+
+Lemma will_fail_subst:
+  forall e ξ,
+    will_fail e = true ->
+    will_fail e.[ξ] = true.
+Proof.
+  intro. remember (size_exp e) as n.
+  assert (size_exp e <= n) by lia. clear Heqn.
+  revert e H.
+  induction n using lt_wf_ind. destruct e; simpl; intros.
+  assumption.
+  destruct e; simpl in *; try assumption.
+  {
+    destruct m; simpl in *; try congruence.
+    destruct e; simpl in *; try congruence.
+    destruct l0; simpl in *; try congruence.
+    destruct f; simpl in *; try congruence.
+    destruct e; simpl in *; try congruence.
+    destruct l0; simpl in *; try congruence.
+    by rewrite length_map.
+  }
+  {
+    apply orb_true_iff in H1 as [H1 | H1]; eapply H in H1; try rewrite H1.
+    all: auto.
+    1,3: lia.
+    by rewrite orb_comm.
+  }
+Qed.
+
+Lemma is_safe_simple_subst:
+  forall e Γ ξ,
+    SUBSCOPE Γ ⊢ ξ ∷ 0 ->
+    EXP Γ ⊢ e ->
+    is_safe_simple e = true ->
+    is_safe_simple e.[ξ] = true.
+Proof.
+  intro. remember (size_exp e) as n.
+  assert (size_exp e <= n) by lia. clear Heqn.
+  revert e H.
+  induction n using lt_wf_ind. destruct e; simpl; intros.
+  * destruct e; simpl in *; try assumption.
+    - inv H2. inv H6. specialize (H1 n0 ltac:(lia)).
+      destruct ξ.
+      + destruct v; try reflexivity. inv H1. lia.
+      + reflexivity.
+    - inv H3.
+  * destruct e; simpl in *; try assumption.
+    - apply andb_true_iff in H3 as [H3_1 H3_2].
+      destruct_scopes.
+      eapply H in H3_1. eapply H in H3_2. by rewrite H3_1, H3_2.
+      all: try eassumption.
+      all: lia.
+    - apply forallb_forall. intros.
+      apply in_map_iff in H4 as [newx [Heq H4]]. subst.
+      eapply forallb_forall in H3. 2: exact H4.
+      eapply H; try eassumption.
+      + pose proof elem_of_list_split l newx.
+        apply elem_of_list_In in H4.
+        apply H5 in H4 as [? [? H4]]. subst l.
+        rewrite map_app, list_sum_app. slia.
+      + apply elem_of_list_In in H4.
+        inv H2. inv H7. apply indexed_to_forall in H6.
+        eapply list.Forall_forall in H6; eassumption.
+    - destruct m; simpl in *; try congruence.
+      destruct e; simpl in *; try congruence.
+      destruct l0; simpl in *; try congruence.
+      destruct f; simpl in *; try congruence.
+      destruct e; simpl in *; try congruence.
+      destruct l0; simpl in *; try congruence.
+      by rewrite length_map.
+Qed.
 
 Lemma closed_seq_elim Γ e :
   EXP Γ ⊢ e -> EXP Γ ⊢ (seq_elim e).
 Proof.
 Admitted.
 
-Lemma will_fail_exception :
-  forall e, will_fail e ->
-    exists exc, ⟨[], e⟩ -->* RExc exc.
+Lemma subst_preserves_size :
+  forall e ξ,
+    size_exp (e.[ξ]) = size_exp e.
 Proof.
-  
+
+Admitted.
+
+Lemma will_fail_exception :
+  forall e res, will_fail e = true ->
+    ⟨[], e⟩ -->* res ->
+    exists exc, res = RExc exc.
+Proof.
+  intro. remember (size_exp e) as n.
+  assert (size_exp e <= n) by lia. clear Heqn.
+  revert e H.
+  induction n using lt_wf_ind. rename H into IH.
+  destruct e; simpl; try congruence.
+  destruct e; simpl; try congruence.
+  * destruct m; simpl; try congruence.
+    destruct e; simpl; try congruence.
+    destruct l0; simpl; try congruence.
+    destruct f; simpl; try congruence.
+    destruct e; simpl; try congruence.
+    destruct l0; simpl; try congruence.
+    intros Hsize ???.
+    destruct H0 as [k [Hres D]].
+    inv D. inv_result.
+    inv H0. inv H1.
+    inv H0. inv H2.
+    inv H0. inv H1.
+    inv H0. inv H2.
+    inv H0. inv H1.
+    unfold is_exit_bif in H. case_match; try congruence.
+    - destruct l; simpl in H; try congruence.
+      destruct l; simpl in H; try congruence.
+      2: destruct l; simpl in H; try congruence.
+      (* single param exception *)
+      + inv H0.
+        pose proof (proj1 (semantic_iff_termination k _ _)
+           (ex_intro _ res (conj Hres H2))) as TERM.
+        apply term_eval_empty in TERM as [rese [ke [Hrese [D Hlt]]]].
+        eapply frame_indep_core in D.
+        pose proof (transitive_eval_rev_lt H2 Hlt D). simpl in H, D.
+        destruct rese; try by inv_result.
+        ** inv H. inv H3.
+           simpl in H11. unfold eval in H11. rewrite H1 in H11.
+           case_match; try congruence.
+           inv H11. inv H6. by eexists. inv H3.
+        ** inv H. inv H3. inv H6. by eexists. inv H.
+      (* two param exception *)
+      + inv H0.
+        pose proof (proj1 (semantic_iff_termination k _ _)
+           (ex_intro _ res (conj Hres H2))) as TERM.
+        apply term_eval_empty in TERM as [rese [ke [Hrese [D Hlt]]]].
+        eapply frame_indep_core in D.
+        pose proof (transitive_eval_rev_lt H2 Hlt D). simpl in H, D.
+        destruct rese; try by inv_result.
+        ** inv H. inv H3.
+           pose proof (proj1 (semantic_iff_termination k0 _ _)
+             (ex_intro _ res (conj Hres H6))) as TERM.
+           apply term_eval_empty in TERM as [rese2 [ke2 [Hrese2 [D2 Hlt2]]]].
+           eapply frame_indep_core in D2.
+           pose proof (transitive_eval_rev_lt H6 Hlt2 D2).
+           simpl in H, D2.
+           destruct rese2; try by inv_result.
+           -- inv H. inv H4.
+              simpl in H13. unfold eval in H13. rewrite H1 in H13.
+              case_match; try congruence.
+              inv H13. inv H8. by eexists. inv H4.
+           -- inv H. inv H4. inv H8. by eexists. inv H.
+        ** inv H. inv H3. inv H6. by eexists. inv H.
+    - destruct l; simpl in H; try congruence.
+      destruct l; simpl in H; try congruence.
+      (* single param exception - as above *)
+      inv H0.
+      pose proof (proj1 (semantic_iff_termination k _ _)
+         (ex_intro _ res (conj Hres H2))) as TERM.
+      apply term_eval_empty in TERM as [rese [ke [Hrese [D Hlt]]]].
+      eapply frame_indep_core in D.
+      pose proof (transitive_eval_rev_lt H2 Hlt D). simpl in H, D.
+      destruct rese; try by inv_result.
+      + inv H. inv H3.
+        simpl in H11. unfold eval in H11. rewrite H1 in H11.
+        case_match; try congruence.
+        inv H11. inv H6. by eexists. inv H3.
+      + inv H. inv H3. inv H6. by eexists. inv H.
+    - destruct l; simpl in H; try congruence.
+      destruct l; simpl in H; try congruence.
+      (* single param exception - as above *)
+      inv H0.
+      pose proof (proj1 (semantic_iff_termination k _ _)
+         (ex_intro _ res (conj Hres H2))) as TERM.
+      apply term_eval_empty in TERM as [rese [ke [Hrese [D Hlt]]]].
+      eapply frame_indep_core in D.
+      pose proof (transitive_eval_rev_lt H2 Hlt D). simpl in H, D.
+      destruct rese; try by inv_result.
+      + inv H. inv H3.
+        simpl in H11. unfold eval in H11. rewrite H1 in H11.
+        case_match; try congruence.
+        inv H11. inv H6. by eexists. inv H3.
+      + inv H. inv H3. inv H6. by eexists. inv H.
+  * intros Hsize ???. case_match; try congruence.
+    destruct H0 as [k [Hres D]].
+    inv D. inv_result.
+    inv H0. inv H2. admit. (* DOABLE, by induction *)
+  * intros. destruct H1 as [k [Hres D]].
+    inv D. inv_result.
+    inv H1.
+    pose proof (proj1 (semantic_iff_termination k0 _ _)
+         (ex_intro _ res (conj Hres H2))) as TERM.
+    apply term_eval_empty in TERM as [rese [ke [Hrese [D Hlt]]]].
+    eapply frame_indep_core in D as D'.
+    pose proof (transitive_eval_rev_lt H2 Hlt D'). simpl in H, D'.
+    apply orb_true_iff in H0 as [|].
+    - simpl in *.
+      specialize (IH (size_exp e1) ltac:(lia) e1 ltac:(lia)
+                     rese H0 (ex_intro _ ke (conj Hrese D))) as [exc Hexc].
+      subst. inv H1. inv H4. inv H7.
+      by eexists.
+      inv H1.
+    - simpl in *. inv Hrese.
+      + inv H1. inv H4.
+        inv H7. by eexists. inv H1.
+      + inv H1. inv H4.
+        ospecialize* (IH (size_exp e2) ltac:(lia) e2.[list_subst vs idsubst] _
+                     res _ (ex_intro _ k (conj Hres H7))).
+        ** rewrite subst_preserves_size. lia.
+        ** by rewrite will_fail_subst.
+        ** assumption.
 Admitted.
 
 Require Import SubstSemanticsLabeled.
 Lemma is_safe_simple_no_effects: 
-  forall e, is_safe_simple e ->
+  forall e, is_safe_simple e = true ->
     exists vs, ⟨[], e⟩  -[ [] ]->ₗ* ⟨[], RValSeq vs⟩.
 Proof.
   
 Admitted.
 
-Lemma eval_seq_optim_1 :
+(* Lemma eval_seq_optim_1 :
   forall e1 e2 res,
    ⟨ [], (° ESeq e1 e2)⟩ -->* res ->
    ⟨ [], (if will_fail (seq_elim e1)
@@ -181,24 +382,102 @@ Lemma eval_seq_optim_2 :
       ⟨ [], (° ESeq e1 e2)⟩ -->* res.
 Proof.
 
-Admitted.
+Admitted. *)
+
+(*
+This won't work, because bodies of binders (e.g., EFun) are not closed!
+
+Theorem seq_optim (e : Exp) :
+  EXPCLOSED e ->
+  CIU e (seq_elim e).
+Proof.
+  remember (size_exp e) as n.
+  assert (size_exp e <= n) by lia. clear Heqn.
+  revert e H.
+  induction n using lt_wf_ind. destruct e; simpl; intros.
+  { apply CIU_iff_Rrel_closed. intros. apply Rrel_Fundamental_closed.
+    scope_solver.  }
+  destruct e; simpl.
+  * apply CIU_iff_Rrel_closed.
+    intros. apply Rrel_exp_compat_closed.
+    apply Erel_Fun_compat_closed.
+    - by destruct_scopes.
+    - apply closed_seq_elim. by destruct_scopes.
+    - eapply H. 2: reflexivity. 2: by destruct_scopes.
+      simpl in H0. lia.
+Qed. *)
+
+(* Lemma seq_elim_subst e ξ: 
+  (seq_elim e).[ξ] = seq_elim (e.[ξ]).
+Proof.
+  remember (size_exp e) as n.
+  assert (size_exp e <= n) by lia. clear Heqn.
+  revert e H ξ.
+  induction n using lt_wf_ind. destruct e; simpl; intros.
+  reflexivity.
+  destruct e; simpl in *; try assumption.
+  * erewrite H. reflexivity. 2: reflexivity. lia.
+  * admit.
+  * admit.
+  * admit.
+  * admit.
+  * admit.
+  * admit.
+  * admit.
+  * admit.
+  * admit.
+  * case_match. 2: case_match. 3: case_match.
+    - eapply will_fail_subst in H1.
+      erewrite H in H1. rewrite H1. 3: reflexivity. 2: lia.
+      erewrite H. reflexivity. 2: reflexivity. lia.
+    - 
+  * admit.
+  * admit.
+Admitted. *)
+
+Lemma CIU_irrefl :
+  forall (e : Exception) (vs : ValSeq),
+    CIU e vs -> False.
+Proof.
+  intros. destruct H as [? [? H]].
+  Check FTry.
+  ospecialize* (H [FTry (length vs) (°inf) 3 (˝VNil)]).
+  * split.
+    - constructor; constructor. constructor. apply inf_scope. do 2 constructor.
+    - constructor; constructor.
+  * eexists. destruct e as [[? ?] ?]. constructor.
+    do 3 constructor.
+  * inv H. inv H2.
+    rewrite eclosed_ignores_sub in H10. 2: constructor; apply inf_scope.
+    by apply inf_diverges in H10.
+Qed.
 
 Theorem seq_optim Γ (e : Exp) :
   EXP Γ ⊢ e ->
-  CIU_open Γ e (seq_elim e).
+  CIU_open Γ e (seq_elim e) /\
+  CIU_open Γ (seq_elim e) e. (* both are needed in the ind hyps. *)
 Proof.
   remember (size_exp e) as n.
   assert (size_exp e <= n) by lia. clear Heqn.
   revert e H Γ.
   induction n using lt_wf_ind. destruct e; simpl; intros.
-  { apply CIU_iff_Rrel. auto. }
+  { split. all: apply CIU_iff_Rrel; auto. }
   pose proof CIU_IsPreCtxRel as CONG.
   destruct e; simpl.
-  * apply CONG; auto.
-    - by destruct_scopes.
-    - apply closed_seq_elim. by destruct_scopes.
-    - eapply H. 2: reflexivity. 2: by destruct_scopes.
-      simpl in H0. lia.
+  * split.
+    { apply CONG; auto.
+      - by destruct_scopes.
+      - apply closed_seq_elim. by destruct_scopes.
+      - eapply H. 2: reflexivity. 2: by destruct_scopes.
+        simpl in H0. lia.
+    }
+    {
+      apply CONG; auto.
+      - apply closed_seq_elim. by destruct_scopes.
+      - by destruct_scopes.
+      - eapply H. 2: reflexivity. 2: by destruct_scopes.
+        simpl in H0. lia.
+    }
   * admit.
   * admit.
   * admit.
@@ -208,17 +487,100 @@ Proof.
   * admit.
   * admit.
   * admit.
-  * split. 2: split.
-    - apply -> subst_preserves_scope_red. 2: exact H2. scope_solver.
-    - apply -> subst_preserves_scope_red. 2: exact H2.
-      repeat case_match.
-      1-3: constructor; apply closed_seq_elim; by destruct_scopes.
-      do 3 constructor;
-      destruct_scopes;
-      by apply closed_seq_elim.
-    - intros. destruct H4.
-      simpl in *.
-
+  * split.
+    {
+      split. 2: split.
+      - apply -> subst_preserves_scope_red. 2: exact H2. scope_solver.
+      - apply -> subst_preserves_scope_red. 2: exact H2.
+        repeat case_match.
+        1-2: constructor; apply closed_seq_elim; by destruct_scopes.
+        do 3 constructor;
+        destruct_scopes;
+        by apply closed_seq_elim.
+      - intros. destruct H4.
+        simpl in *.
+        inv H4. 2: inv_result.
+        case_match.
+        2: case_match.
+        {
+          eapply will_fail_subst in H4 as H4'.
+          pose proof will_fail_exception (seq_elim e1).[ξ] H4' as [exc D1].
+          destruct D1 as [n1 [Hres1 D1]].
+          pose proof (H (size_exp e1) ltac:(lia) e1 ltac:(lia) Γ
+            ltac:(by destruct_scopes)) as [CIUe1_1 CIUe1_2].
+          specialize (CIUe1_1 _ H2) as [_ [_ D3]].
+          simpl in D3. destruct H3.
+          ospecialize *(D3 (FSeq e2.[ξ]::F)).
+          { split. constructor. 2: assumption.
+            * constructor.
+              clear -H1 H2.
+              destruct_scopes.
+              apply -> subst_preserves_scope_exp; eassumption.
+            * constructor. constructor. assumption. }
+          { eexists. exact H9. }
+          destruct D3.
+          eapply frame_indep_nil in D1 as D1'.
+          eapply term_step_term in H6. 2: exact D1'.
+          inv H6.
+          eexists.
+          eapply step_term_term_plus.
+          eapply frame_indep_nil in D1. exact D1.
+          exact H13.
+        }
+        {
+          eapply is_safe_simple_subst with (ξ := ξ) in H5.
+          apply is_safe_simple_no_effects in H5 as D.
+          destruct D as [vs [k1 D]].
+          apply step_rt_labeled_to_unlabeled in D.
+          pose proof (H (size_exp e1) ltac:(lia) e1 ltac:(lia) Γ
+            ltac:(by destruct_scopes)) as [CIUe1_1 CIUe1_2].
+          eapply term_eval_empty in H9 as D'.
+          destruct D' as [res [k1' [Hres [D' Hlt]]]].
+          pose proof (CIUe1_1 _ H2).
+          pose proof (CIUe1_2 _ H2).
+          assert (CIU res vs /\ CIU vs res). {
+            clear -D D' H6 H7 H1 H2.
+            apply CIU_eval_base in D' as [].
+            2: { destruct_scopes. constructor.
+                 apply -> subst_preserves_scope_exp; eassumption.
+            }
+            apply CIU_eval_base in D as [].
+            2: { destruct_scopes. constructor.
+                 apply -> subst_preserves_scope_exp; try eassumption.
+                 by apply closed_seq_elim.
+            }
+            split.
+            * pose proof (CIU_transitive_closed _ _ _ H0 H6).
+              pose proof (CIU_transitive_closed _ _ _ H5 H3).
+              assumption.
+            * pose proof (CIU_transitive_closed _ _ _ H7 H).
+              pose proof (CIU_transitive_closed _ _ _ H4 H5).
+              assumption.
+          }
+          eapply frame_indep_core in D'.
+          epose proof term_step_term _ _ _ _ H9 _ _ D'.
+          2: eassumption.
+          2: apply closed_seq_elim; by destruct_scopes.
+          simpl in *.
+          destruct res; try by inv_result.
+          2: {
+            destruct H8 as [C1 C2].
+            clear -C1. exfalso.
+            by apply CIU_irrefl in C1.
+          }
+          inv H10.
+          apply ex_intro with (x := k0) in H12.
+          pose proof (H (size_exp e2) ltac:(lia) e2 ltac:(lia) Γ
+            ltac:(by destruct_scopes)) as [CIUe2_1 CIUe2_2].
+          eapply CIUe2_1; eassumption.
+        }
+        {
+          
+        }
+      }
+      {
+        admit.
+      }
   * admit.
   * admit.
 Admitted.
